Remastered OrdSet, added useful lemmas and utils

ulib/experimental/FStar.OrdSet.fst
@@ -18,19 +18,74 @@ module FStar.OrdSet
 type ordset a f = l:(list a){sorted f l}
 
 let hasEq_ordset _ _ = ()
-
-val as_list (#a:eqtype) (#f:cmp a) (s:ordset a f) : Tot (l:list a{sorted f l})
-let as_list #_ #_ s = s
-
+    
+let rec simple_induction #t #f (p: ordset t f -> Type0) (x: ordset t f)
+  : Lemma (requires p [] /\ (forall (l: ordset t f{Cons? l}). p (Cons?.tl l) ==> p l))
+          (ensures p x) = match x with
+  | [] -> ()
+  | ph::pt -> simple_induction p pt;
+            assert (p (Cons?.tl (ph::pt)))
+  
+let rec base_induction #t #f (p: ordset t f -> Type0) (x: ordset t f)
+  : Lemma (requires (forall (l: ordset t f{List.Tot.Base.length l < 2}). p l) 
+                  /\ (forall (l: ordset t f{Cons? l}). p (Cons?.tl l) ==> p l))
+          (ensures p x) 
+          (decreases List.Tot.Base.length x) = 
+  if List.Tot.Base.length x < 2 then ()
+  else match x with
+  | ph::pt -> base_induction p pt;
+            assert (p (Cons?.tl (ph::pt)))
+            
 let empty #_ #_ = []
 
+let tail #a #f s = Cons?.tl s <: ordset a f 
+let head #_ #_ s = Cons?.hd s
+
 let mem #_ #_ x s = List.Tot.mem x s
+ 
+(* In case snoc-based List implementation is optimized, we use library ones,
+   but we additionally supply them with relevant postconditions that come 
+   from s being an ordset. *)
+let rec last_direct #a #f (s: ordset a f{s <> empty}) 
+  : (x:a{mem x s /\ (forall (z:a{mem z s}). f z x)}) 
+  = match s with
+  | [x] -> x  
+  | h::g::t -> last_direct (tail s)
+
+let last_lib #a #f (s: ordset a f{s <> empty}) 
+  = snd (List.Tot.Base.unsnoc s)
+
+let last_eq #a #f (s: ordset a f{s <> empty}) 
+  : Lemma (last_direct s = last_lib s) = simple_induction 
+    (fun p -> if p<>[] then last_direct #a #f p = last_lib p else true) s
+
+let last #a #f s = last_eq s; last_lib s
+
+let rec liat_direct #a #f (s: ordset a f{s <> empty}) : (l:ordset a f{
+    (forall x. mem x l = (mem x s && (x <> last s))) /\
+    (if tail s <> empty then head s = head l else true)
+  }) =  
+  match s with
+  | [x] -> []
+  | h::g::t -> h::(liat_direct #a #f (g::t))
+
+let liat_lib #a #f (s: ordset a f{s <> empty}) = fst (List.Tot.Base.unsnoc s)
+
+let liat_eq #a #f (s:ordset a f {s<>empty})
+  : Lemma (liat_direct s = liat_lib s) = simple_induction
+    (fun p -> if p<>[] then liat_direct p = liat_lib p else true) s
+
+let liat #a #f s = liat_eq s; liat_lib s
+
+let unsnoc #a #f s = liat s, last s
+
+let as_list (#a:eqtype) (#f:cmp a) (s:ordset a f) : Tot (l:list a{sorted f l}) = s
 
 val insert': #a:eqtype -> #f:cmp a -> x:a -> s:ordset a f
              -> Tot (l:(ordset a f){let s = as_list s in let l = as_list l in
 	                           (Cons? l /\
-                                    (Cons?.hd l = x \/
-                                    (Cons? s /\ Cons?.hd l = Cons?.hd s)))})
+                                    (head #a #f l = x \/
+                                    (Cons? s /\ head #a #f l = head #a #f s)))})
 let rec insert' #_ #f x s =
   match s with
   | []     -> [x]
@@ -41,143 +96,93 @@ let rec insert' #_ #f x s =
 
 let rec union #_ #_ s1 s2 = match s1 with
   | []     -> s2
-  | hd::tl -> union tl (insert' hd s2)
-
-let rec intersect #a #f s1 s2 = match s1 with
-  | []     -> []
-  | hd::tl ->
-    if mem #_ #f hd s2 then
-      insert' #_ #f hd (intersect #_ #f tl s2)
-    else
-      intersect #_ #f tl s2
-
-let choose #a #f s = match s with
-  | []   -> None
-  | x::_ -> Some x
+  | hd::tl -> union tl (insert' hd s2) 
 
 val remove': #a:eqtype -> #f:cmp a -> x:a -> s:ordset a f
-             -> Tot (l:(ordset a f){let s = as_list s in let l = as_list l in
-	                           ((Nil? s ==> Nil? l) /\
-                                    (Cons? s ==> Cons?.hd s = x ==> l = Cons?.tl s) /\
-                                    (Cons? s ==> Cons?.hd s =!= x ==> (Cons? l /\ Cons?.hd l = Cons?.hd s)))})
+             -> Tot (l:(ordset a f){ ((Nil? s ==> Nil? l) /\
+                                    (Cons? s ==> head s = x ==> l = tail s) /\
+                                    (Cons? s ==> head s =!= x ==> (Cons? l /\ head l = Cons?.hd s)))})
+                                    
 let rec remove' #a #f x s = match s with
-  | []     -> []
-  | hd::tl ->
-    if x = hd then tl
-    else hd::(remove' #_ #f x tl)
-
-let remove #a #f x s = remove' #_ #f x s
-
-let size #a #f s = List.Tot.length s
-
-let rec subset #a #f s1 s2 = match s1, s2 with
-  | [], _          -> true
-  | hd::tl, hd'::tl' ->
-    if f hd hd' && hd = hd' then subset #a #f tl tl'
-    else if f hd hd' && not (hd = hd') then false
-    else subset #a #f s1 tl'
-  | _, _           -> false
-
-let singleton (#a:eqtype) #f x = [x]
- 
-private
-let rec remove_le #a #f x (s:ordset a f)
-  : Pure (ordset a f)
-    (requires True)
-    (ensures (fun r -> let r = as_list r in sorted f (x :: r)))
-    (decreases s)
-=
-  match s with
   | [] -> []
-  | y :: ys -> if f x y && x <> y
-             then s
-             else remove_le #a #f x ys
+  | hd::(tl: ordset a f) ->
+    if x = hd then tl
+    else hd::(remove' x tl)
 
-let rec not_mem_aux #a #f x (s:ordset a f)
-  : Lemma (requires (size s > 0) && (Cons?.hd s <> x) && (f x (Cons?.hd s)))
-          (ensures not (mem x s))
-          = 
-  match s with  
-  | h::t -> if t = [] then () else not_mem_aux #a #f x t 
+let size' (#a:eqtype) (#f:cmp a) (s:ordset a f) = List.Tot.length s
 
-let rec tail_is_subset #a #f (s:ordset a f{size s > 0})
-  : Lemma (Cons?.tl s `subset` s) = 
-  match s with
-  | [] -> ()
-  | h::(t:ordset a f) -> if size t > 0 then tail_is_subset #a #f t
+let liat_length #a #f (s:ordset a f{s<>empty}) : Lemma (size' (liat s) = ((size' s) - 1)) 
+  = simple_induction (fun p -> if p<>empty then size' (liat p) = ((size' p)-1) else true) s
 
-let rec self_is_subset #a #f (s:ordset a f)
-  : Lemma (subset s s) = match s with 
-  | [] -> ()
-  | h::(t:ordset a f) -> self_is_subset t
+let rec not_mem_aux (#a:eqtype) (#f:cmp a) (x:a) (s:ordset a f)
+  : Lemma (requires (size' s > 0) && (head s <> x) && (f x (head s)))
+          (ensures not (mem x s)) = 
+  if tail s <> [] then not_mem_aux x (tail s)
 
+let rec subset' #a #f (s1 s2: ordset a f) = match s1, s2 with
+  | [], _          -> true
+  | hd::tl, hd'::tl' -> if f hd hd' && hd = hd' then subset' #a #f tl tl'
+                     else if f hd hd' && not (hd = hd') then false
+                     else subset' #a #f s1 tl'
+  | _, _           -> false
+  
+let tail_is_subset #a #f (s:ordset a f{size' s > 0})
+  : Lemma (Cons?.tl s `subset'` s) = 
+  simple_induction (fun (s:ordset a f) -> size' s=0 || subset' (Cons?.tl s) s) s
+  
+let self_is_subset #a #f (s:ordset a f)
+  : Lemma (subset' s s) = simple_induction (fun (s:ordset a f) -> subset' s s) s
+
+(* 
+  returns a pair of (fst z) = (everything from s that goes after x)
+  and (snd z) = (true if x was found in s, false otherwise)
+*)
 let rec remove_until_greater_than #a #f x (s: ordset a f)
-  : z:(ordset a f * bool) { (size (fst z) <= size s) &&
-                            not(mem x (fst z)) &&
-                            (subset (fst z) s) &&
+  : z:(ordset a f * bool) { (size' (fst z) <= size' s) &&
+                            (not(mem x (fst z))) &&
+                            (subset' (fst z) s) &&
                             (snd z = mem x s) &&
                             (match (fst z) with 
-                            | [] -> true
-                            | h::t -> (sorted f (x::(fst z)))) } =
+                             | [] -> true
+                             | h::t -> (sorted f (x::(fst z)))) 
+                          } =
   match s with
   | [] -> ([], false)
-  | h::(t:ordset a f) -> if h=x then (
-                        assert (sorted f t);   
-                        if size t > 0 then not_mem_aux x t;
-                        tail_is_subset s;
-                        (t, true)
-                      )
-          else if f x h then (
-            not_mem_aux x s;
-            self_is_subset s;
-            (s, false)
-          )
-          else remove_until_greater_than x t
-
+  | h::(t:ordset a f) -> if h=x then begin
+                         if size' t > 0 then not_mem_aux x t;
+                         tail_is_subset s;
+                         (t, true)
+                       end
+                       else if f x h then begin
+                         not_mem_aux x s;
+                         self_is_subset s;
+                       (s, false)
+                       end 
+                       else remove_until_greater_than x t
 
 let rec remove_until_gt_prop #a #f (s: ordset a f) (x:a) (test:a)
   : Lemma (f test x ==> not (mem test (fst (remove_until_greater_than x s)))) = 
   match s with
   | [] -> ()
   | h::(t:ordset a f) -> 
-          let aux (test:a) 
-            : Lemma (requires f test x && h<>test) 
-                    (ensures not (mem test (fst (remove_until_greater_than x s)))) =
-            remove_until_gt_prop #a #f t x test;
-            () in Classical.move_requires aux test;
-          if h <> x then remove_until_gt_prop t x test
+    let aux (test:a) : Lemma (requires f test x && h<>test) 
+                             (ensures not (mem test (fst (remove_until_greater_than x s)))) =
+      remove_until_gt_prop #a #f t x test 
+    in Classical.move_requires aux test;
+    if h <> x then remove_until_gt_prop t x test
 
 let rec remove_until_gt_mem #a #f (s: ordset a f) (x:a) (test:a)
   : Lemma (mem test (fst (remove_until_greater_than x s)) = (
              mem test s &&
              f x test &&
              (x<>test)
-           )) = 
-  match s with
-  | [] -> ()
-  | h::(t:ordset a f) -> remove_until_gt_prop s x test;
-                       remove_until_gt_mem t x test
+           )) 
+  = if size' s > 0 then remove_until_gt_mem (tail s) x test
 
-
-let mem_of_empty #a #f (s: ordset a f{size s = 0}) (x: a)
-  : Lemma (not (mem x s)) = ()
-
-let rec mem_implies_f #a #f (s: ordset a f) (x:a)
-  : Lemma (requires mem x s) (ensures f (Cons?.hd s) x) = 
-  match s with 
-  | [] -> ()
-  | h::t -> if size s > 0 && x <> h then mem_implies_f #a #f t x
-
-let mem_of_tail #a #f (s: ordset a f{size s > 0}) (x:a)
-  : Lemma ((mem #a #f x (Cons?.tl s) || (x = Cons?.hd s)) = mem x s) = ()
-
-let not_mem_of_tail #a #f (s: ordset a f{size s > 0}) (x:a)
-  : Lemma ((not (mem #a #f x (Cons?.tl s))) = (not (mem x s) || (x = Cons?.hd s))) = 
- match s with
- | h::[] -> ()
- | h::g::t -> if x = h then Classical.move_requires (mem_implies_f #a #f (g::t)) x 
-           else mem_of_tail s x 
-
+let mem_implies_f #a #f (s: ordset a f) (x:a)
+  : Lemma (requires mem x s) (ensures f (Cons?.hd s) x) 
+  = simple_induction (fun s -> mem x s ==> f (head s) x) s
+    
 (* 
    Smart intersect is the set intersect that accounts for the ordering of both lists,
    eliminating some checks by trimming leading elements of one of the input lists 
@@ -189,7 +194,7 @@ let rec smart_intersect #a #f (s1 s2: ordset a f) : Tot (z:ordset a f{
     (forall x. mem x z = (mem x s1 && mem x s2)) /\
     (forall (x:a{sorted f (x::s1)}). sorted f (x::z)) /\
     (forall (x:a{sorted f (x::s2)}). sorted f (x::z)) 
-  }) (decreases size s1 + size s2) = 
+  }) (decreases size' s1 + size' s2) = 
   match s1 with 
   | [] -> []
   | h1::(t1:ordset a f) -> match s2 with
@@ -213,80 +218,77 @@ let rec smart_intersect #a #f (s1 s2: ordset a f) : Tot (z:ordset a f{
         )
       end
 
-val set_props_aux:
-  #a:eqtype -> #f:cmp a -> s:ordset a f{Cons? (as_list s)}
-  -> Lemma (requires True)
-          (ensures  (let s = as_list s in
-	             (forall x. List.Tot.mem x (Cons?.tl s) ==> (f (Cons?.hd s) x /\ Cons?.hd s =!= x))))
-                     
-let rec set_props_aux (#a:eqtype) #f s = match s with
-  | x::tl -> if tl = [] then () else set_props_aux #a #f tl
+let intersect #a #f s1 s2 = smart_intersect s1 s2
+
+let choose #a #f s = match s with | [] -> None | x::_ -> Some x
+  
+let remove #a #f x s = remove' #_ #f x s
+
+let size #a #f s = size' s
+
+let subset #a #f s1 s2 = subset' s1 s2
+
+let singleton (#a:eqtype) #f x = [x]
+
+let mem_of_empty #a #f (s: ordset a f{size s = 0}) (x: a)
+  : Lemma (not (mem x s)) = ()
+
+let mem_of_tail #a #f (s: ordset a f{size s > 0}) (x:a)
+  : Lemma ((mem #a #f x (Cons?.tl s) || (x = Cons?.hd s)) = mem x s) = ()
+
+let not_mem_of_tail #a #f (s: ordset a f{size s > 0}) (x:a)
+  : Lemma (not (mem x (tail s)) = not (mem x s) || x = head s) 
+  = simple_induction (fun s -> mem x s ==> f (head s) x) s
+
+let rec set_props #a #f (s:ordset a f) 
+  : Lemma (if size s > 0 then ((forall x. mem x (tail s) ==> f (head s) x /\ head s <> x)) 
+           else forall x. not (mem x s))
+  = if (size s > 1) then set_props (tail s)
 
 let rec same_members_means_eq #a #f (s1 s2: ordset a f)
-  : Lemma (requires forall x. mem x s1 = mem x s2) (ensures s1 == s2) = 
+  : Lemma (requires forall x. mem x s1 = mem x s2) (ensures s1 = s2) = 
   match s1 with
-  | [] -> if size s2>0 then assert (mem #a #f (Cons?.hd s2) s2) 
-  | h1::t1 -> set_props_aux s1;
-            set_props_aux s2;
+  | [] -> if size s2>0 then assert (mem (head s2) s2) 
+  | h1::t1 -> set_props s1;
+            set_props s2;
             match s2 with 
             | h2::t2 -> same_members_means_eq #a #f t1 t2 
 
-let intersect_sym #a #f (s1 s2: ordset a f) 
-  : Lemma (smart_intersect s1 s2 = smart_intersect s2 s1) = 
-  same_members_means_eq (smart_intersect s1 s2) (smart_intersect s2 s1)
+let intersect_is_symmetric #a #f (s1 s2: ordset a f) 
+  : Lemma (smart_intersect s1 s2 = smart_intersect s2 s1) 
+  = same_members_means_eq (smart_intersect s1 s2) (smart_intersect s2 s1)
 
 let remove_until_gt_exclusion #a #f (s:ordset a f) (x:a) (test:a)
   : Lemma (requires f x test && (not (mem test (fst (remove_until_greater_than x s)))))
           (ensures x=test || not (mem test s)) = 
   remove_until_gt_mem s x test 
-    
-let rec remove_le_removes_x #a #f x (s:ordset a f)
-  : Lemma (not (mem x (fst (remove_until_greater_than x s)))) = 
-  match s with
-  | y::ys -> remove_le_removes_x #a #f x ys
+      
+let rec mem_implies_subset #a #f (s1 s2: ordset a f)
+  : Lemma ((forall x. mem x s1 ==> mem x s2) ==> subset s1 s2)
+  = match s1 with 
   | [] -> ()
+  | h1::(t1:ordset a f) -> set_props s1;
+                         set_props s2;
+                         mem_implies_subset t1 s2;
+                         if (size s2 > 0 && f (head s2) h1) 
+                         then mem_implies_subset s1 (tail s2)
 
-
-val mem_implies_subset_aux:
-  #a:eqtype -> #f:cmp a -> s1:ordset a f -> s2:ordset a f
-  -> Lemma (requires (True))
-          (ensures ((forall x. mem #a #f x s1 ==> mem #a #f x s2) ==> subset #a #f s1 s2))
-          
-let rec mem_implies_subset_aux (#a:eqtype) #f s1 s2 = match s1, s2 with
-  | [], [] -> ()
-  | _::_, [] -> ()
-  | [], _::_ -> ()
-  | hd::tl, hd'::tl' ->
-    set_props_aux #a #f s1; set_props_aux #a #f s2;
-
-    if f hd hd' && hd = hd' then
-      mem_implies_subset_aux #a #f tl tl'
-    else if f hd hd' && not (hd = hd') then
-      ()
-    else mem_implies_subset_aux #a #f s1 tl'
-
-val subset_implies_mem_aux:
-  #a:eqtype -> #f:cmp a -> s1:ordset a f -> s2:ordset a f
-  -> Lemma (requires (True))
-          (ensures (subset #a #f s1 s2 ==> (forall x. mem #a #f x s1 ==>
-                                                mem #a #f x s2)))
-let rec subset_implies_mem_aux (#a:eqtype) #f s1 s2 = match s1, s2 with
-  | [], _          -> ()
-  | hd::tl, hd'::tl' ->
-    if f hd hd' && hd = hd' then subset_implies_mem_aux #a #f tl tl'
-    else subset_implies_mem_aux #a #f s1 tl'
-  | _, _           -> ()
-
+let rec subset_implies_mem #a #f (p q: ordset a f)
+  : Lemma (subset p q ==> (forall x. mem x p ==> mem x q)) = 
+ if Cons? p && Cons? q then 
+   if head p = head q
+   then subset_implies_mem (tail p) (tail q)
+   else subset_implies_mem p (tail q)
+ 
 let subset_transitivity #a #f (p q r: ordset a f)
   : Lemma (requires p `subset` q /\ q `subset` r)
           (ensures p `subset` r) = 
-  subset_implies_mem_aux p q;
-  subset_implies_mem_aux q r;
-  mem_implies_subset_aux p r
-
+  subset_implies_mem p q;
+  subset_implies_mem q r;
+  mem_implies_subset p r
 
 let head_is_never_in_tail #a #f (s:ordset a f{size s > 0}) 
-  : Lemma (not (mem #a #f (Cons?.hd s) (Cons?.tl s))) = set_props_aux s
+  : Lemma (not (mem (head s) (tail s))) = set_props s
 
 let rec smart_minus #a #f (p q: ordset a f) 
   : z:ordset a f { ( forall x. mem x z = (mem x p && (not (mem x q)))) /\
@@ -305,37 +307,24 @@ let rec smart_minus #a #f (p q: ordset a f)
       Classical.forall_intro (Classical.move_requires (mem_implies_f p));  
       if found then begin
         let result = smart_minus pt q_after_ph in
-        set_props_aux p;
-        if result = [] then begin
+        set_props p;
+        if result = [] then begin          
           subset_transitivity pt q_after_ph q;
-          subset_implies_mem_aux pt q;          
-          mem_implies_subset_aux p q
+          subset_implies_mem pt q;          
+          mem_implies_subset p q
         end;
         result
       end
       else ph::(smart_minus pt q_after_ph)      
 
-let minus_empty_means_subset #a #f (p q: ordset a f)
+let empty_minus_means_subset #a #f (p q: ordset a f)
   : Lemma (requires size (smart_minus p q) = 0) (ensures subset p q) = ()
 
+// a little test versus integers :)
 let ncmp (x y:nat) = x <= y
-
 let _ = assert (smart_minus #nat #ncmp [1;2;3;4] [3] == [1;2;4])
   
 let minus #a #f s1 s2 = smart_minus s1 s2 
-
-let rec remove_le_never_increases_size #a #f (s: ordset a f) (x:a)
-  : Lemma (size (remove_le x s) <= size s) = 
-  match s with
-  | [] -> ()
-  | h::t -> remove_le_never_increases_size #a #f t x
-
-let rec remove_le_decreases_size #a #f (s: ordset a f) (x:a)
-  : Lemma (requires mem x s) (ensures size (remove_le x s) < size s) = 
-  match s with
-  | [] -> ()
-  | h::t -> if x=h then () else remove_le_decreases_size #a #f t x
-    
 
 let minus_removes_s2 #a #f (p q: ordset a f) (x:a)
   : Lemma (ensures mem x q ==> not (mem x (minus p q))) = ()
@@ -343,158 +332,76 @@ let minus_removes_s2 #a #f (p q: ordset a f) (x:a)
 let minus_removes_all_of_s2 #a #f (s1 s2: ordset a f) (x:a{mem x s2})
   : Lemma (not (mem x (minus s1 s2))) = ()  
 
-let strict_subset #a #f s1 s2 = s1 <> s2 && subset #a #f s1 s2
+let strict_subset #a #f s1 s2 = s1 <> s2 && subset s1 s2
 
-val set_props:
-  #a:eqtype -> #f:cmp a -> s:ordset a f{Cons? (as_list s)}
-  -> Lemma (requires True)
-          (ensures  (let s = as_list s in
-	             (forall x. List.Tot.mem x (Cons?.tl s) ==> (f (Cons?.hd s) x /\ Cons?.hd s =!= x))))
-let rec set_props (#a:eqtype) #f s = match s with
-  | x::tl -> if tl = [] then () else set_props #a #f tl
+let hd_unique #a #f (s: ordset a f) 
+  : Lemma (requires size s > 0) 
+          (ensures not (mem (head s) (tail s))) = set_props s
 
-val hd_unique: #a:eqtype -> #f:cmp a -> s:ordset a f
-               -> Lemma (requires (Cons? (as_list s)))
-                       (ensures (let s = as_list s in
-		                 not (List.Tot.mem (Cons?.hd s) (Cons?.tl s))))
-let hd_unique #a #f s = set_props #a #f s
-
-val eq_helper: #a:eqtype -> #f:cmp a -> x:a -> s:ordset a f
-               -> Lemma (requires (let s = as_list s in Cons? s /\ f x (Cons?.hd s) /\ x =!= Cons?.hd s))
-                       (ensures (not (mem #a #f x s)))
-let eq_helper (#a:eqtype) #f x s = set_props #a #f s
-
-let rec eq_lemma (#a:eqtype) #f s1 s2 = match s1, s2 with
-  | [], []             -> ()
-  | _::_, []           -> ()
-  | [], _::_           -> ()
-  | hd1::tl1, hd2::tl2 ->
-    if hd1 = hd2 then
-      //hd_unique calls help us prove that forall x. mem f x tl1 = mem f x tl2
-      //so that we can apply IH
-      (hd_unique #_ #f s1; hd_unique #_ #f s2; eq_lemma #_ #f tl1 tl2)
-    else if f hd1 hd2 then
-      eq_helper #_ #f hd1 s2
-    else
-      eq_helper #_ #f hd2 s1
+let eq_lemma #a #f s1 s2 = same_members_means_eq s1 s2
 
 let mem_empty #_ #_ _ = ()
 
 let mem_singleton #_ #_ _ _ = ()
 
-val insert_mem: #a:eqtype -> #f:cmp a -> x:a -> y:a -> s:ordset a f
-                -> Lemma (requires (True))
-                         (ensures (mem #a #f y (insert' #a #f x s) =
-                                   (x = y || mem #a #f y s)))
-let rec insert_mem (#a:eqtype) #f x y s = match s with
-  | []     -> ()
-  | hd::tl ->
-    if x = hd then ()
-    else if f x hd then ()
-    else insert_mem #_ #f x y tl
+let mem_insert (#a:eqtype) #f (el:a) (s: ordset a f) (x:a)
+  : Lemma (mem x (insert' el s) = (x=el || mem x s)) = 
+  simple_induction (fun p -> mem x (insert' el p) = (x=el || mem x p)) s
+  
+let rec mem_union #_ #_ s1 s2 x = 
+  if size s1 > 0 then 
+    match s1 with | hd::tl -> 
+      mem_union tl (insert' hd s2) x;
+      mem_insert hd s2 x
 
-let rec mem_union #_ #f x s1 s2 = match s1 with
-  | []     -> ()
-  | hd::tl ->
-    mem_union #_ #f x tl (insert' #_ #f hd s2); insert_mem #_ #f hd x s2
-
-let rec mem_intersect #_ #f x s1 s2 = match s1 with
-  | []     -> ()
-  | hd::tl ->
-    let _ = mem_intersect #_ #f x tl s2 in
-    if mem #_ #f hd s2 then insert_mem #_ #f hd x (intersect #_ #f tl s2) else ()
-
-val subset_implies_mem:
-  #a:eqtype -> #f:cmp a -> s1:ordset a f -> s2:ordset a f
-  -> Lemma (requires (True))
-          (ensures (subset #a #f s1 s2 ==> (forall x. mem #a #f x s1 ==>
-                                                mem #a #f x s2)))
-let rec subset_implies_mem (#a:eqtype) #f s1 s2 = match s1, s2 with
-  | [], _          -> ()
-  | hd::tl, hd'::tl' ->
-    if f hd hd' && hd = hd' then subset_implies_mem #a #f tl tl'
-    else subset_implies_mem #a #f s1 tl'
-  | _, _           -> ()
-
-val mem_implies_subset:
-  #a:eqtype -> #f:cmp a -> s1:ordset a f -> s2:ordset a f
-  -> Lemma (requires (True))
-          (ensures ((forall x. mem #a #f x s1 ==> mem #a #f x s2) ==> subset #a #f s1 s2))
-let rec mem_implies_subset (#a:eqtype) #f s1 s2 = match s1, s2 with
-  | [], [] -> ()
-  | _::_, [] -> ()
-  | [], _::_ -> ()
-  | hd::tl, hd'::tl' ->
-    set_props #a #f s1; set_props #a #f s2;
-
-    if f hd hd' && hd = hd' then
-      mem_implies_subset #a #f tl tl'
-    else if f hd hd' && not (hd = hd') then
-      ()
-    else mem_implies_subset #a #f s1 tl'
+let mem_intersect #_ #f s1 s2 x = ()
 
 let mem_subset (#a:eqtype) #f s1 s2 =
-  subset_implies_mem #a #f s1 s2; mem_implies_subset #a #f s1 s2
+  subset_implies_mem s1 s2; 
+  mem_implies_subset s1 s2
 
 let choose_empty (#a:eqtype) #f = ()
 
-let choose_s (#a:eqtype) #f s =
-  let Some e = choose #_ #f s in
-  cut (equal #a #f s (insert' #a #f e (remove #a #f e s)))
+let choose_s (#a:eqtype) #f s = () 
 
-let rec mem_remove (#a:eqtype) #f x y s = match s with
-  | []     -> ()
-  | hd::tl -> if y = hd then hd_unique #_ #f s else mem_remove #_ #f x y tl
+let rec mem_remove (#a:eqtype) #f x y s = 
+  if size s > 0 then (hd_unique s; mem_remove x y (tail s))
 
-let rec eq_remove (#a:eqtype) #f x s = match s with
-  | []    -> ()
-  | _::tl -> eq_remove #_ #f x tl
+let eq_remove (#a:eqtype) #f x s 
+  = simple_induction (fun p -> not (mem x p) ==> p = remove x p) s
 
 let size_empty (#a:eqtype) #f s = ()
 
 let rec size_remove (#a:eqtype) #f x s = match s with
-  | hd::tl ->
-    if x = hd then () else size_remove #_ #f x tl
+  | hd::tl -> if x<>hd then size_remove #_ #f x tl
 
 let size_singleton (#a:eqtype) #f x = ()
 
 let rec subset_size (#a:eqtype) #f x y = match x, y with
   | [], _          -> ()
-  | hd::tl, hd'::tl' ->
-    if f hd hd' && hd = hd' then subset_size #a #f tl tl'
-    else subset_size #a #f x tl'
-
-(**********)
-
-let singleton_union_sym (#a:eqtype) #f (s: ordset a f) (x:a) 
-  : Lemma (ensures union s [x] == union [x] s)
-          (decreases s) = eq_lemma (union s [x]) (union [x] s)
-
-let rec insert_when_already_exists (#a:eqtype) #f (s: ordset a f) (x:a)
-  : Lemma (requires mem x s) (ensures insert' x s == s) = 
-  match s with
-  | h::t -> if h<>x then insert_when_already_exists #a #f t x
-  | [] -> ()
-
-let rec size_insert (#a:eqtype) #f (s: ordset a f) (x:a)
-  : Lemma (size (insert' x s) >= size s) = 
-  match s with 
-  | h::t -> size_insert #a #f t x
-  | [] -> ()
-
+  | hd::tl, hd'::(tl':ordset a f) ->
+    if f hd hd' && hd = hd' then subset_size tl tl'
+    else subset_size x tl'
+  
+let insert_when_already_exists (#a:eqtype) #f (s: ordset a f) (x:a)
+  : Lemma (requires mem x s) 
+          (ensures insert' x s == s)  
+  = simple_induction (fun p -> mem x p <==> insert' x p = p) s
+  
+let size_insert (#a:eqtype) #f (s: ordset a f) (x:a)
+  : Lemma (size (insert' x s) >= size s) 
+  = simple_induction (fun p -> size (insert' x p) >= size p) s
+  
 let rec precise_size_insert (#a:eqtype) #f (s: ordset a f) (x:a)
-  : Lemma (ensures size (insert' x s) = (if mem x s then size s else (size s) + 1)) = 
-  match s with
-  | h::t -> precise_size_insert #a #f t x
-  | [] -> ()
+  : Lemma (size (insert' x s) = (if mem x s then size s else (size s) + 1)) 
+  = if size s > 0 then precise_size_insert (tail s) x
        
 let rec size_of_union_left (#a:eqtype) #f (s1 s2: ordset a f)
-  : Lemma (ensures size (union s1 s2) >= size s2) =
+  : Lemma (ensures size (union s1 s2) >= size s2) = 
   match s1 with
   | [] -> ()
-  | hd::tl -> size_of_union_left #a #f tl (insert' hd s2);
-            precise_size_insert s2 hd;
-            if mem hd s2 then insert_when_already_exists s2 hd 
+  | hd::tl -> size_of_union_left tl (insert' hd s2);
+            precise_size_insert s2 hd
 
 let size_of_union_right (#a:eqtype) #f (s1 s2: ordset a f)
   : Lemma (ensures size (union s1 s2) >= size s1) =
@@ -504,16 +411,14 @@ let size_of_union_right (#a:eqtype) #f (s1 s2: ordset a f)
 let size_union #a #f s1 s2 =
   size_of_union_left s1 s2;
   size_of_union_right s1 s2
-
-(**********)
-
+ 
 let fold #a #acc #f g init s = List.Tot.fold_left g init s
 
 private
 let rec map_internal (#a #b:eqtype) (#fa:cmp a) (#fb:cmp b) (g:a -> b) (sa:ordset a fa)
   : Pure (ordset b fb)
     (requires (forall x y. x `fa` y ==> g x `fb` g y))
-    (ensures (fun sb -> let sa = as_list sa in let sb = as_list sb in Cons? sb ==> Cons? sa /\ Cons?.hd sb == g (Cons?.hd sa)))
+    (ensures (fun sb -> Cons? sb ==> Cons? sa /\ Cons?.hd sb == g (Cons?.hd sa)))
 = match sa with
   | [] -> []
   | x :: xs ->
@@ -523,146 +428,165 @@ let rec map_internal (#a #b:eqtype) (#fa:cmp a) (#fb:cmp b) (g:a -> b) (sa:ordse
       y :: ys
     else ys
 
-let map #a #b #fa #fb g sa = map_internal #a #b #fa #fb g sa
+let rec map_size (#a #b:eqtype) (#fa:cmp a) (#fb: cmp b) (g: a->b) (sa:ordset a fa)
+  : Lemma (requires (forall x y. x `fa` y ==> g x `fb` g y))
+          (ensures size (map_internal #a #b #fa #fb g sa) <= size sa) 
+  = if size sa > 0 then map_size #a #b #fa #fb g (tail sa)
+
+let map #a #b #fa #fb g sa = 
+  map_size #a #b #fa #fb g sa;
+  map_internal #a #b #fa #fb g sa
 
 let lemma_strict_subset_size #a #f s1 s2 = 
   let eql (p q: ordset a f) 
     : Lemma (requires forall x. mem x p = mem x q) 
             (ensures p=q) 
-    = eq_lemma p q in 
-  Classical.move_requires_2 eql s1 s2;
+    = eq_lemma p q in Classical.move_requires_2 eql s1 s2;
   eliminate exists x. mem x s2 && not (mem x s1) 
   returns size s2 > size s1 with _.
   begin
-    let ins_mem x s p // perhaps we should reorder parameters of insert_mem...
-      : Lemma(mem p (insert' x s) = (p=x || mem p s)) 
-      = insert_mem x p s in
-    Classical.forall_intro (ins_mem x s1);
+    Classical.forall_intro (mem_insert x s1);
     precise_size_insert s1 x;
     assert (subset (insert' x s1) s2)
   end
-
-let aux_lemma_remove (#a:eqtype) #f (s: ordset a f) (x:a) (test:a)
-  : Lemma (mem test (remove x s) = (mem test s && not (x=test))) = ()
-
-let remove_le_empty #a #f x (s:ordset a f) : Lemma (requires s = empty) (ensures remove_le #a #f x s = empty) = ()
- 
-let me_empty (#a:eqtype) (#f:cmp a) (x:a) (s1 s2:ordset a f)
-  : Lemma (requires sorted f (x::s1) /\ sorted f (x::s2) /\ s2=empty) 
-          (ensures s1 = (minus s1 s2)) = ()
-
-let minus_empty (#a:eqtype) #f (s1 s2: ordset a f) : Lemma (requires s2=empty) (ensures minus s1 s2 = s1) = ()
-    
+   
 let lemma_minus_mem #a #f s1 s2 x = ()
-
-
+ 
 let rec strict_subset_implies_diff_element #a #f (s1 s2: ordset a f) 
   : Lemma (requires strict_subset s1 s2)
           (ensures exists x. (mem x s2 /\ not (mem x s1))) = 
   match s1,s2 with
   | [], h::t -> ()
-  | h1::t1, h2::t2 -> if h1<>h2 then (
-                     if f h2 h1 then Classical.move_requires (mem_implies_f s1) h2 
-                   ) else begin
+  | h1::t1, h2::t2 -> Classical.move_requires (mem_implies_f s1) h2;
+                   if h1=h2 then begin
                      strict_subset_implies_diff_element #a #f t1 t2; 
-                     not_mem_of_tail s2 h1 
+                     set_props s2                     
                    end
 
 let diff_element_implies_strict_subset #a #f (s1 s2: ordset a f)
   : Lemma (requires subset s1 s2 /\ (exists x. (mem x s2 /\ not (mem x s1))))
           (ensures strict_subset s1 s2) = ()
 
-let diff_element_equals_strict_subset #a #f (s1 s2: ordset a f)
+let lemma_strict_subset_exists_diff #a #f (s1 s2: ordset a f)
   : Lemma (requires subset s1 s2)
           (ensures (strict_subset s1 s2) <==> (exists x. (mem x s2 /\ not (mem x s1)))) 
   = Classical.move_requires_2 strict_subset_implies_diff_element s1 s2
-
-let rec count #a #f (s: ordset a f) (condition: a -> bool) : nat = 
+ 
+let rec count #a #f s c : nat = 
   match s with
   | [] -> 0
-  | h::t -> if condition h 
-          then 1 + count #a #f t condition 
-          else count #a #f t condition
+  | h::t -> if c h 
+          then 1 + count #a #f t c 
+          else count #a #f t c
 
-let rec count_of_impossible_is_zero #a #f (s:ordset a f) (condition: a -> bool {forall p. not (condition p)}) 
-  : Lemma (count s condition = 0) = 
-  match s with 
-  | [] -> ()
-  | h::t -> count_of_impossible_is_zero #a #f t condition 
+let count_of_empty #_ #_ _ _ = ()
 
-let rec count_all #a #f (s: ordset a f) : Lemma (count s (fun x -> true) = size s) = 
+let count_of_impossible #a #f s c = simple_induction (fun p -> count p c = 0) s
+
+let count_all #a #f s c = simple_induction (fun p -> count p c = size p) s
+
+let rec count_of_cons #a #f s c = if size s > 1 then count_of_cons (tail s) c 
+
+let rec all #a #f (s: ordset a f) (c: condition a) : Tot bool = 
   match s with
-  | [] -> ()
-  | h::t -> count_all #a #f t
+  | [] -> true
+  | h::t -> c h && all #a #f t c
 
-let intersect_with_empty #a #f (s: ordset a f) 
-  : Lemma (smart_intersect s [] = [] /\ smart_intersect [] s = []) = ()
+let rec any #a #f (s: ordset a f) (c: condition a) : Tot bool = 
+  match s with
+  | [] -> false
+  | h::t -> c h || any #a #f t c
 
-let size_of_tail #a #f (s:ordset a f) 
-  : Lemma (requires size s > 0)
-          (ensures size s = 1 + (size #a #f (Cons?.tl s))) = ()
+let rec mem_if_any #a #f s c x = if head s<>x then mem_if_any (tail s) c x
 
-let count_of_empty #a #f (s: ordset a f) 
-  : Lemma (requires size s = 0) (ensures forall (c: a -> bool). count s c = 0) = () 
+let any_if_mem #a #f (s:ordset a f) (c: condition a) x
+  : Lemma (requires mem x s && c x) (ensures any s c) = 
+  simple_induction (fun p -> mem x p && c x ==> any p c) s
+ 
+let all_means_not_any_not #a #f s c = simple_induction (fun p -> all p c = not (any p (inv c))) s
 
-let count_of_tail #a #f (s: ordset a f{size s > 0}) (r: ordset a f{size r > 0})
-  : Lemma (requires Cons?.hd s = Cons?.hd r)
-          (ensures count s (fun x -> mem x r) = 1 + count #a #f (Cons?.tl s) (fun x -> mem x r)) = () 
+let rec find_first #a #f s c = match s with
+  | [] -> None
+  | h::(t:ordset a f) -> if c h then Some h else find_first t c
 
-let rec where #a #f (s: ordset a f) (cond: a -> bool) 
-  : Pure (ordset a f) 
-         (requires True)
-         (ensures fun (z:ordset a f) -> 
-           (forall x. mem x z = (mem x s && cond x)) /\
-           (if size z > 0 && size s > 0 then f (Cons?.hd s) (Cons?.hd z) else true) )= 
+let find_first_is_some_iff_any #_ #_ s c = simple_induction (fun p -> Some? (find_first p c) = any p c) s
+ 
+let rec find_first_precedes_any_other #a #f s c x =   
+  if head s<>x then find_first_precedes_any_other (tail s) c x;
+  set_props s
+
+let liat_size #a #f (s:ordset a f{s<>[]}) : Lemma (size (liat s) = size s - 1) = 
+  base_induction (fun p -> if p<>[] then size (liat p) = size p - 1 else true) s
+
+let mem_liat #a #f (s:ordset a f{s<>[]}) (x:a)
+  : Lemma (mem x s = (mem x (liat s) || x = last s)) = ()
+
+let rec any_liat #a #f (s:ordset a f{s<>[]}) (c: condition a)
+  : Lemma (any s c = (any (liat s) c || c (last s))) = match s with
+  | [x] -> ()
+  | h::(t:ordset a f) -> if size t > 0 then any_liat t c
+
+let rec find_last' #a #f (s: ordset a f) (c: condition a) : Tot (option a) (decreases size s) =
+  if s=empty then None 
+  else let liat,last = unsnoc s in
+    liat_size s;
+    if c last then Some last
+    else find_last' liat c
+
+let rec find_last_props #a #f (s:ordset a f) (c: condition a)
+  : Lemma (ensures (match find_last' s c with
+           | None -> not (any s c)
+           | Some v -> (any s c /\ (forall (x:a{mem x s && c x}). f x v))))
+          (decreases size s) =
+  if size s > 0 then let liat,last = unsnoc s in
+    liat_size s;     
+    find_last_props liat c; 
+    if c last then any_if_mem s c last else any_liat s c  
+
+let find_last #a #f s c = 
+  find_last_props s c;
+  find_last' s c
+
+let find_last_is_some_iff_any #a #f s c = find_last_props s c
+
+let find_last_follows_any_other #a #f s c x = 
+  any_if_mem s c x; 
+  find_last_is_some_iff_any s c;
+  find_last_props s c
+  
+let size_of_tail #a #f s  = ()
+ 
+let count_of_tail #_ #_ _ _ = () 
+
+let rec where #a #f s c = 
   match s with
   | [] -> []
-  | h::[] -> if cond h then [h] else []
-  | h::g::[] -> if cond h then h::(where #a #f [g] cond) else where #a #f [g] cond
-  | h::g::(t:ordset a f) -> if cond h then h::(where #a #f (g::t) cond) else where (g::t) cond 
+  | h::[] -> if c h then [h] else []
+  | h::(t:ordset a f) -> if c h then h::(where t c) else where t c 
+ 
+let intersect_eq_where #_ #_ s1 s2 = 
+  same_members_means_eq (where s1 (mem_of s2)) (intersect s1 s2)
 
-let intersect_eq_where #a #f (s1 s2: ordset a f)
-  : Lemma (smart_intersect s1 s2 = where s1 (fun x -> mem x s2)) = 
-  let rhs = where s1 (fun x -> mem x s2) in
-  let lhs = smart_intersect s1 s2 in 
-  same_members_means_eq lhs rhs
+let minus_eq_where #_ #_ s1 s2 = 
+  same_members_means_eq (where s1 (inv (mem_of s2))) (minus s1 s2)
 
-let minus_eq_where #a #f (s1 s2: ordset a f)
-  : Lemma (smart_minus s1 s2 = where s1 (fun x -> not (mem x s2))) = 
-  let rhs = where s1 (fun x -> not (mem x s2)) in
-  let lhs = smart_minus s1 s2 in 
-  same_members_means_eq lhs rhs  
+let count_is_size_of_where #_ #_ s c 
+  = simple_induction (fun p -> count p c = size (where p c)) s
 
-let rec count_is_size_of_where #a #f (s: ordset a f) (cond: a -> bool)
-  : Lemma (count s cond = size (where s cond)) = 
-  match s with
-  | [] -> ()
-  | h::t -> count_is_size_of_where #a #f t cond
-
-let size_of_intersect #a #f (s1 s2: ordset a f)
-  : Lemma (ensures size (smart_intersect s1 s2) = count s1 (fun x -> mem x s2) /\
-                   size (smart_intersect s1 s2) = count s2 (fun x -> mem x s1))
-          (decreases size s1 + size s2) =   
+let size_of_intersect #_ #_ s1 s2 =    
   intersect_eq_where s1 s2;
   intersect_eq_where s2 s1;
-  intersect_sym s1 s2;
-  count_is_size_of_where s1 (fun x -> mem x s2);   
-  count_is_size_of_where s2 (fun x -> mem x s1)
-  
-let count_of_intersect #a #f (s1 s2: ordset a f) 
-  : Lemma (count s1 (fun x -> mem x s2) = count s2 (fun x -> mem x s1)) = size_of_intersect s1 s2
-
+  intersect_is_symmetric s1 s2;
+  count_is_size_of_where s1 (mem_of s2);   
+  count_is_size_of_where s2 (mem_of s1)
+    
 let union_mem_forall #a #f (s1 s2: ordset a f)
   : Lemma (forall x. (mem x (union s1 s2)) = (mem x s1 || mem x s2)) =
   let aux x : Lemma (mem x (union s1 s2) = (mem x s1 || mem x s2)) =   
-    mem_union x s1 s2 in Classical.forall_intro aux  
+    mem_union s1 s2 x in Classical.forall_intro aux  
 
-let union_with_empty #a #f (s: ordset a f)
-  : Lemma (union s empty = s) = 
-  let aux x : Lemma (mem x (union s empty) = mem x s) =   
-    mem_union x s empty in
-  Classical.forall_intro aux;
-  eq_lemma (union s empty) s
+let union_with_empty #a #f (s: ordset a f) 
+  : Lemma (union s empty = s) = eq_lemma (union s empty) s
 
 let union_head_lemma #a #f (s1 s2: ordset a f)
   : Lemma (match s1, s2 with 
@@ -708,84 +632,86 @@ let union_of_tails_size (#a:eqtype) #f (s1 s2: ordset a f)
     set_props s2;
     same_members_means_eq (h1::(union t1 s2)) (union s1 s2)
 
+let union_is_symmetric #a #f (s1 s2: ordset a f) : Lemma (union s1 s2 = union s2 s1) = 
+  same_members_means_eq (union s1 s2) (union s2 s1)
+
 #push-options "--z3rlimit 10"
-let rec size_of_union #a #f (s1 s2: ordset a f)
-  : Lemma (ensures size (union s1 s2) = size s1 + size s2 - (size (smart_intersect s1 s2)))
+let rec size_of_union #a #f s1 s2 
+  : Lemma (ensures size (union s1 s2) = (size s1 + size s2 - size (smart_intersect s1 s2)))
           (decreases size s1 + size s2) = 
   let size = size #a #f in
   match s1,s2 with
-  | [], _ -> union_mem_forall s1 s2;
-            same_members_means_eq s2 (union s1 s2)
+  | [], _ -> union_mem_forall s1 s2
   | _, [] -> union_mem_forall s1 s2;
             same_members_means_eq s1 (union s1 s2)
-  | h1::(t1:ordset a f), h2::(t2:ordset a f) -> size_of_union #a #f t1 t2;
-                   assert (size (union t1 t2) = size t1 + size t2 - size (smart_intersect t1 t2));
-                   if h1 = h2 then union_with_prefix h1 t1 t2
-                   else if f h1 h2 then begin
-                     size_of_union t1 s2;
-                     union_of_tails_size s1 s2;
-                     Classical.move_requires (mem_implies_f s2) h1;
-                     same_members_means_eq (smart_intersect s1 s2) (smart_intersect t1 s2)
-                   end else begin
-                     size_of_union s1 t2;
-                     intersect_sym s1 t2;
-                     same_members_means_eq (union s1 s2) (union s2 s1);
-                     same_members_means_eq (union s1 t2) (union t2 s1); 
-                     union_of_tails_size s2 s1; 
-                     same_members_means_eq (smart_intersect s1 s2) (smart_intersect t2 s1)
-                   end 
+  | h1::(t1:ordset a f), h2::(t2:ordset a f) 
+          -> size_of_union #a #f t1 t2;
+            assert (size (union t1 t2) = size t1 + size t2 - size (smart_intersect t1 t2));
+            if h1 = h2 then union_with_prefix h1 t1 t2
+            else if f h1 h2 then begin 
+              size_of_union t1 s2;
+              union_of_tails_size s1 s2;
+              Classical.move_requires (mem_implies_f s2) h1;
+              same_members_means_eq (smart_intersect s1 s2) (smart_intersect t1 s2)
+            end else begin 
+              size_of_union s1 t2;
+              intersect_is_symmetric s1 t2;
+              same_members_means_eq (union s1 s2) (union s2 s1);
+              same_members_means_eq (union s1 t2) (union t2 s1); 
+              union_of_tails_size s2 s1; 
+              same_members_means_eq (smart_intersect s1 s2) (smart_intersect t2 s1)
+            end 
 #pop-options
 
-let rec count_dichotomy #a #f (s: ordset a f) (cond: a -> bool)
-  : Lemma (size s = count s cond + count s (fun x -> not (cond x))) = 
-  match s with
-  | [] -> ()
-  | h::t -> count_dichotomy #a #f t cond
+let rec count_dichotomy #_ #_ s c = if s<>[] then count_dichotomy (tail s) c
 
-let size_of_minus #a #f (s1 s2: ordset a f)
-  : Lemma (size (smart_minus s1 s2) = size s1 - size (smart_intersect s1 s2)) = 
+let size_of_minus #_ #_ s1 s2 =
   minus_eq_where s1 s2;
-  intersect_eq_where s1 s2;
-  let mem_of_s2 x = mem x s2 in
-  let not_mem_of_s2 x = not (mem x s2) in
-  count_dichotomy s1 mem_of_s2; 
-  count_is_size_of_where s1 mem_of_s2;
-  count_is_size_of_where s1 not_mem_of_s2
+  intersect_eq_where s1 s2; 
+  count_dichotomy s1 (mem_of s2); 
+  count_is_size_of_where s1 (mem_of s2);
+  count_is_size_of_where s1 (inv (mem_of s2))
  
-let intersect_with_subset #a #f (s1 s2: ordset a f)
-  : Lemma (requires subset s1 s2)
-          (ensures smart_intersect s1 s2 = s1) = 
-  same_members_means_eq (smart_intersect s1 s2) s1
+let intersect_with_subset #_ #_ s1 s2 = same_members_means_eq (intersect s1 s2) s1
  
-let lemma_strict_subset_minus_size #a #f s1 s2 s = 
+let lemma_strict_subset_minus_size #_ #_ s1 s2 s = 
   let size_diff : pos = size s2 - size s1 in
-  size_of_minus s2 s1;
   size_of_minus s s2;
   size_of_minus s s1;
   intersect_with_subset s2 s;
-  intersect_sym s2 s;
+  intersect_is_symmetric s2 s;
   intersect_with_subset s1 s;
-  intersect_sym s1 s
+  intersect_is_symmetric s1 s
 
-let lemma_disjoint_union_subset #a #f s1 s2 = size_of_union s1 s2
+let lemma_disjoint_union_subset #_ #_ s1 s2 = size_of_union s1 s2
 
-let lemma_subset_union #a #f s1 s2 s = ()
+let lemma_subset_union #_ #_ _ _ _ = ()
 
-let lemma_strict_subset_transitive #a #f s1 s2 s3 = ()
+let lemma_strict_subset_transitive #_ #_ _ _ _ = ()
 
-let lemma_intersect_symmetric #a #f s1 s2 = eq_lemma (intersect s1 s2) (intersect s2 s1)
+let lemma_intersect_symmetric = intersect_is_symmetric
 
-let lemma_intersect_union_empty #a #f s1 s2 s3 = eq_lemma empty (intersect (union s1 s2) s3)
+let lemma_intersect_union_empty_aux1 #a #f (s1 s2 s3: ordset a f) 
+  : Lemma (requires (intersect s1 s3 == empty /\ intersect s2 s3 == empty))
+          (ensures (intersect (union s1 s2) s3 = empty))
+  = eq_lemma empty (intersect (union s1 s2) s3)
 
-let lemma_intersect_union_empty' #a #f s1 s2 s3 = eq_lemma empty (intersect s1 s3);
-                                                  eq_lemma empty (intersect s2 s3) 
+let lemma_intersect_union_empty_aux2 #a #f (s1 s2 s3: ordset a f)  
+  : Lemma (requires (intersect (union s1 s2) s3 = empty))
+          (ensures (intersect s1 s3 == empty /\ intersect s2 s3 == empty))  
+  = eq_lemma empty (intersect s1 s3);
+    eq_lemma empty (intersect s2 s3) 
 
-let union_comm #a #f s1 s2 = eq_lemma (union s1 s2) (union s2 s1)
+let lemma_intersect_union_empty #a #f (s1 s2 s3: ordset a f)
+  : Lemma ((intersect (union s1 s2) s3 = empty) = 
+           (intersect s1 s3 = empty && intersect s2 s3 = empty))
+    [SMTPat (intersect (union s1 s2) s3)] =  
+  Classical.move_requires_3 (lemma_intersect_union_empty_aux1 #a #f) s1 s2 s3;
+  Classical.move_requires_3 (lemma_intersect_union_empty_aux2 #a #f) s1 s2 s3
 
-let union_of_disj #a #f s1 s2 = 
-  let aux x : Lemma (mem x (minus (union s1 s2) s1) = (mem x s2)) 
-    = mem_intersect x s1 s2 in Classical.forall_intro aux;
-  eq_lemma (minus (union s1 s2) s1) s2
+let lemma_union_symmetric #a #f s1 s2 = eq_lemma (union s1 s2) (union s2 s1)
+
+let union_of_disjoint #a #f s1 s2 = eq_lemma (minus (union s1 s2) s1) s2
 
 (* Conversion from OrdSet to Set *)
 
@@ -804,10 +730,16 @@ let rec lemma_as_set_mem #a #f s x
         then ()
         else lemma_as_set_mem #a #f tl x
 
-let rec lemma_as_set_disjoint #a #f s1 s2
-  = match s1 with
-    | []     -> ()
-    | hd::tl ->
-        if mem hd s2
-        then assert (S.mem hd (as_set s2))
-        else lemma_as_set_disjoint tl s2
+let lemma_as_set_disjoint_right #a #f (s1 s2: ordset a f)
+  : Lemma (requires intersect s1 s2 = empty)
+          (ensures S.disjoint (as_set s1) (as_set s2)) = ()
+
+let lemma_as_set_disjoint_left #a #f (s1 s2: ordset a f)
+  : Lemma (requires S.disjoint (as_set s1) (as_set s2)) 
+          (ensures intersect s1 s2 = empty) =     
+  let mem_eq p q : Lemma (S.mem p (as_set q) <==> mem #a #f p q) = () in
+  Classical.forall_intro_2 mem_eq
+
+let lemma_as_set_disjoint #a #f s1 s2 = 
+  Classical.move_requires_2 (lemma_as_set_disjoint_right #a #f) s1 s2;
+  Classical.move_requires_2 (lemma_as_set_disjoint_left #a #f) s1 s2
